common/Common.ProtocolImplementation.fst
@@ -7,21 +7,113 @@ open Pulse.Lib.Pervasives
 module P = Common.Protocol
 module TCP = Common.TCP
 
+type parsed_messages (wire_message:Type0) =
+  option (list wire_message & TCP.bytes)
+
 noextract
 class protocol_implementation
   (impl:Type0)
   (state:Type0)
   (wire_message:Type0)
   (event:Type0)
+  (network_args:Type0)
+  (network_result:Type0)
+  (local_args:Type0)
+  (local_result:Type0)
   =
 {
   pi_protocol:
     P.state_machine_protocol state wire_message event;
 
-  pi_represents:
+  pi_parse_network:
+    TCP.bytes -> GTot (parsed_messages wire_message);
+
+  pi_serialize_network:
+    wire_message -> GTot (option TCP.bytes);
+
+  pi_serialized_network:
+    wire_message ->
+    TCP.bytes ->
+    GTot prop;
+
+  pi_parse_network_correct:
+    bytes:TCP.bytes ->
+      Lemma
+        (ensures
+          (match pi_parse_network bytes with
+          | None -> True
+          | Some (msgs, residual) ->
+            pi_protocol.P.sm_wire_format.P.wf_stream_matches
+              P.NetworkReceived
+              bytes
+              msgs
+              residual));
+
+  pi_serialize_network_correct:
+    msg:wire_message ->
+      Lemma
+        (ensures
+          (match pi_serialize_network msg with
+          | None -> True
+          | Some bytes ->
+            pi_serialized_network msg bytes));
+
+  pi_tcp_channel:
+    impl ->
+    TCP.history ->
+    slprop;
+
+  pi_ghost_log:
+    impl ->
+    state ->
+    slprop;
+
+  pi_runtime_resources:
     impl ->
     state ->
     TCP.history ->
     slprop;
-}
 
+  pi_invariant:
+    impl ->
+    state ->
+    TCP.history ->
+    slprop;
+
+  pi_invariant_correct:
+    state ->
+    TCP.history ->
+    GTot prop;
+
+  pi_network_pre:
+    impl ->
+    network_args ->
+    slprop;
+
+  pi_network_post:
+    impl ->
+    network_args ->
+    network_result ->
+    slprop;
+
+  pi_local_pre:
+    impl ->
+    local_args ->
+    slprop;
+
+  pi_local_post:
+    impl ->
+    local_args ->
+    local_result ->
+    slprop;
+
+  pi_network_signature:
+    impl ->
+    network_args ->
+    GTot Type0;
+
+  pi_local_signature:
+    impl ->
+    local_args ->
+    GTot Type0;
+}
